a single canonical ctx_rel for our languages

theories/simulang/behavior.v
@@ -1,64 +1,62 @@
-From iris.proofmode Require Import tactics.
-From iris.base_logic Require Import iprop.
-From iris.prelude Require Import options.
-
+From stdpp Require Import gmap.
+From iris.prelude Require Import prelude.
 From simuliris.logic Require Import satisfiable.
 From simuliris.simulation Require Import behavior.
 From simuliris.simulang Require Import lang notation wf gen_val_rel.
 
-(** Define "observable behavior" and a generic notion of contextual refinement.
-*)
-Section ctx_rel.
-  Context (expr_head_wf : expr_head → Prop).
+From iris.prelude Require Import options.
 
-  (** We currently don't allow global variables that initially contain
-  pointers. However, this is not a real restriction as [main] can
-  store pointers in global variables. (In fact, it would be good
-  enough to 0-initialize all global variables.) *)
-  Definition init_state (σ_t σ_s : state) : Prop :=
-    ∃ gs, map_Forall (λ _ v, val_wf v) gs ∧ σ_t = state_init gs ∧ σ_s = state_init gs.
+(** Define "observable behavior" and contextual refinement. *)
 
-  Fixpoint obs_val (v_t v_s : val) {struct v_s} : Prop :=
-    match v_t, v_s with
-    | LitV (LitLoc l_t), LitV (LitLoc l_s) =>
-      True (* the details of locations are not observable *)
-    | LitV l_t, LitV l_s =>
-      l_t = l_s
-    | PairV v1_t v2_t, PairV v1_s v2_s =>
-      obs_val v1_t v1_s ∧ obs_val v2_t v2_s
-    | InjLV v_t, InjLV v_s =>
-      obs_val v_t v_s
-    | InjRV v_t, InjRV v_s =>
-      obs_val v_t v_s
-    | _,_ => False
-    end.
+(** We currently don't allow global variables that initially contain
+pointers. However, this is not a real restriction as [main] can
+store pointers in global variables. (In fact, it would be good
+enough to 0-initialize all global variables.) *)
+Definition init_state (σ_t σ_s : state) : Prop :=
+  ∃ gs, map_Forall (λ _ v, val_wf v) gs ∧ σ_t = state_init gs ∧ σ_s = state_init gs.
 
-  (** The simulang instance of [beh_rel]. *)
-  Definition beh_rel := beh_rel init_state "main" #() obs_val.
+Fixpoint obs_val (v_t v_s : val) {struct v_s} : Prop :=
+  match v_t, v_s with
+  | LitV (LitLoc l_t), LitV (LitLoc l_s) =>
+    True (* the details of locations are not observable *)
+  | LitV l_t, LitV l_s =>
+    l_t = l_s
+  | PairV v1_t v2_t, PairV v1_s v2_s =>
+    obs_val v1_t v1_s ∧ obs_val v2_t v2_s
+  | InjLV v_t, InjLV v_s =>
+    obs_val v_t v_s
+  | InjRV v_t, InjRV v_s =>
+    obs_val v_t v_s
+  | _,_ => False
+  end.
 
-  (** Contextual refinement:
-      The two [e] can be put into an arbitrary context in an arbitrary function.
-      [λ: x, e] denotes an evaluation context [let x = <hole> in e]; then the
-      <hole> will be the function argument. *)
-  Definition gen_ctx_rel (e_t e_s : expr) :=
-    ∀ (C : ctx) (fname x : string) (p : prog),
-      (* The other functions need to be well-formed and closed *)
-      map_Forall (λ _ '(arg, body), gen_expr_wf expr_head_wf body ∧ free_vars body ⊆ {[arg]}) p →
-      (* The context needs to be well-formed *)
-      gen_ctx_wf expr_head_wf C →
-      (* The context needs to close our expressions *)
-      free_vars (fill_ctx C e_t) ∪ free_vars (fill_ctx C e_s) ⊆ {[x]} →
-      (* Then we demand [beh_rel] if putting our expressions into a context to
-         obtain a whole function and that function into a program *)
-      beh_rel (<[fname := (x, fill_ctx C e_t)]> p) (<[fname := (x, fill_ctx C e_s)]> p).
+(** The simulang instance of [beh_rel]. *)
+Definition beh_rel := beh_rel init_state "main" #() obs_val.
 
-  Lemma gen_val_rel_obs {Σ} loc_rel v_t v_s :
-    gen_val_rel loc_rel v_t v_s ⊢@{iPropI Σ} ⌜obs_val v_t v_s⌝.
-  Proof.
-    iInduction v_t as [[| | | | |]| | |] "IH" forall (v_s);
-      destruct v_s as [[| | | | |]| | |]; try by eauto.
-    - simpl. iIntros "[Hv1 Hv2]". iSplit.
-      + by iApply "IH".
-      + by iApply "IH1".
-  Qed.
-End ctx_rel.
+(** Default well-formedness for SimuLang. *)
+Definition simulang_wf (e : expr_head) : Prop :=
+  match e with
+  | ValHead v => val_wf v
+  (* Na2Ord is an intermediate (administrative) ordering that should only
+       arise during execution and programs should not use it directly. *)
+  | LoadHead o => o ≠ Na2Ord
+  | StoreHead o => o ≠ Na2Ord
+  | _ => True
+  end.
+
+Notation expr_wf := (gen_expr_wf simulang_wf).
+Notation ectx_wf := (gen_ectx_wf simulang_wf).
+Notation ctx_wf := (gen_ctx_wf simulang_wf).
+
+(** Contextual refinement. *)
+Definition ctx_rel (e_t e_s : expr) :=
+  ∀ (C : ctx) (fname x : string) (p : prog),
+    (* The other functions need to be well-formed and closed *)
+    map_Forall (λ _ '(arg, body), expr_wf body ∧ free_vars body ⊆ {[arg]}) p →
+    (* The context needs to be well-formed *)
+    ctx_wf C →
+    (* The context needs to close our expressions *)
+    free_vars (fill_ctx C e_t) ∪ free_vars (fill_ctx C e_s) ⊆ {[x]} →
+    (* Then we demand [beh_rel] if putting our expressions into a context to
+       obtain a whole function and that function into a program *)
+    beh_rel (<[fname := (x, fill_ctx C e_t)]> p) (<[fname := (x, fill_ctx C e_s)]> p).
