theories/stacked_borrows/behavior.v
@@ -1,80 +1,58 @@
-From iris.proofmode Require Import tactics.
-From iris.base_logic Require Import iprop.
+From stdpp Require Import gmap.
+From iris.prelude Require Import prelude.
+From simuliris.simulation Require Import behavior.
+From simuliris.stacked_borrows Require Import defs wf.
 From iris.prelude Require Import options.
 
-From simuliris.logic Require Import satisfiable.
-From simuliris.simulation Require Import behavior.
-From simuliris.stacked_borrows Require Import lang notation parallel_subst wf logical_state.
+(** Define "observable behavior" and contextual refinement. *)
 
-(* TODO move to std++ *)
-Lemma Forall2_cons_iff {A B} (P : A → B → Prop)
-  (x : A) (l : list A) (y : B) (k : list B) :
-  Forall2 P (x :: l) (y :: k) ↔ P x y ∧ Forall2 P l k.
-Proof.
-  split.
-  - apply Forall2_cons_inv.
-  - intros []. by apply Forall2_cons.
-Qed.
+(** Force initial state to be empty *)
+Definition init_state (σ_t σ_s : state) : Prop :=
+  σ_t = init_state ∧ σ_s = init_state.
 
-(** Define "observable behavior" and a generic notion of contextual refinement.
-*)
-Section ctx_rel.
-  Context (expr_head_wf : expr_head → Prop).
+Definition obs_scalar (sc_t sc_s : scalar) :=
+  match sc_t, sc_s with
+  | ScPtr l1 t1, ScPtr l2 t2 => True (* the details of locations are not observable *)
+  | ScInt z1, ScInt z2 => z1 = z2
+  | ScFnPtr f1, ScFnPtr f2 => f1 =f2
+  | ScCallId c1, ScCallId c2 => c1 = c2
+  | _, ScPoison => True (* anything is compatibl with "poison" in the source *)
+  | _, _ => False
+  end
+.
+Definition obs_value (v_t v_s : value) : Prop := Forall2 obs_scalar v_t v_s.
+Definition obs_result (r_t r_s : val bor_lang) : Prop :=
+  match r_t, r_s with
+  | PlaceR _ _ _, PlaceR _ _ _ =>
+    True (* the details of locations are not observable *)
+  | ValR v_t, ValR v_s => obs_value v_t v_s
+  | _, _ => False
+  end.
 
-  (** Force initial state to be empty *)
-  Definition init_state (σ_t σ_s : state) : Prop :=
-    σ_t = init_state ∧ σ_s = init_state.
+(** The Stacked Borrows instance of [beh_rel]. *)
+Definition beh_rel := beh_rel init_state "main" (ValR [ScPoison]) obs_result.
 
-  Definition obs_scalar (sc_t sc_s : scalar) :=
-    match sc_t, sc_s with
-    | ScPtr l1 t1, ScPtr l2 t2 => True (* the details of locations are not observable *)
-    | ScInt z1, ScInt z2 => z1 = z2
-    | ScFnPtr f1, ScFnPtr f2 => f1 =f2
-    | ScCallId c1, ScCallId c2 => c1 = c2
-    | _, ScPoison => True (* anything is compatibl with "poison" in the source *)
-    | _, _ => False
-    end
-    .
-  Definition obs_value (v_t v_s : value) : Prop := Forall2 obs_scalar v_t v_s.
-  Definition obs_result (r_t r_s : val bor_lang) : Prop :=
-    match r_t, r_s with
-    | PlaceR _ _ _, PlaceR _ _ _ =>
-      True (* the details of locations are not observable *)
-    | ValR v_t, ValR v_s => obs_value v_t v_s
-    | _, _ => False
-    end.
+(** Default well-formedness for Stacked Borrows *)
+Definition stackedborrows_wf (e : expr_head) : Prop :=
+  match e with
+  | ValHead v => value_wf v
+  | PlaceHead _ _ _ => False (* no literal pointers *)
+  | _ => True
+  end.
 
-  (** The Stacked Borrows instance of [beh_rel]. *)
-  Definition beh_rel := beh_rel init_state "main" (ValR [ScPoison]) obs_result.
+Notation expr_wf := (gen_expr_wf stackedborrows_wf).
+Notation ectx_wf := (gen_ectx_wf stackedborrows_wf).
+Notation ctx_wf := (gen_ctx_wf stackedborrows_wf).
 
-  (** Contextual refinement:
-      The two [e] can be put into an arbitrary context in an arbitrary function.
-      [λ: x, e] denotes an evaluation context [let x = <hole> in e]; then the
-      <hole> will be the function argument. *)
-  Definition gen_ctx_rel (e_t e_s : expr) :=
-    ∀ (C : ctx) (fname x : string) (p : prog),
-      map_Forall (λ _ '(arg, body), gen_expr_wf expr_head_wf body ∧ free_vars body ⊆ {[arg]}) p →
-      gen_ctx_wf expr_head_wf C →
-      free_vars (fill_ctx C e_t) ∪ free_vars (fill_ctx C e_s) ⊆ {[x]} →
-      beh_rel (<[fname := (x, fill_ctx C e_t)]> p) (<[fname := (x, fill_ctx C e_s)]> p).
-
-  Lemma sc_rel_obs `{!sborGS Σ} sc_t sc_s :
-    sc_rel sc_t sc_s ⊢@{iPropI Σ} ⌜ obs_scalar sc_t sc_s ⌝.
-  Proof.
-    destruct sc_t, sc_s; try by eauto.
-    rewrite sc_rel_cid_source. iIntros "[<- _]". eauto.
-  Qed.
-
-  Lemma rrel_obs `{!sborGS Σ} r_t r_s :
-    rrel r_t r_s ⊢@{iPropI Σ} ⌜ obs_result r_t r_s ⌝.
-  Proof.
-    destruct r_t as [v_t|], r_s as [v_s|]; try by eauto.
-    iInduction v_t as [|sc_t scs_t] "IH" forall (v_s);
-      destruct v_s as [|sc_s scs_s]; simpl; try eauto.
-    { iIntros "_ !%". constructor. }
-    rewrite {2}/value_rel big_sepL2_cons.
-    iIntros "[Hs Hss]". rewrite /obs_value Forall2_cons_iff. iSplit.
-    - iApply (sc_rel_obs with "Hs").
-    - iApply ("IH" with "Hss").
-  Qed.
-End ctx_rel.
+(** Contextual refinement *)
+Definition ctx_rel (e_t e_s : expr) :=
+  ∀ (C : ctx) (fname x : string) (p : prog),
+    (* The other functions need to be well-formed and closed *)
+    map_Forall (λ _ '(arg, body), expr_wf body ∧ free_vars body ⊆ {[arg]}) p →
+    (* The context needs to be well-formed *)
+    ctx_wf C →
+    (* The context needs to close our expressions *)
+    free_vars (fill_ctx C e_t) ∪ free_vars (fill_ctx C e_s) ⊆ {[x]} →
+    (* Then we demand [beh_rel] if putting our expressions into a context to
+       obtain a whole function and that function into a program *)
+    beh_rel (<[fname := (x, fill_ctx C e_t)]> p) (<[fname := (x, fill_ctx C e_s)]> p).
