theories/simulang/na_inv/examples/data_races.v
@@ -1,8 +1,8 @@
 From iris Require Import bi.bi.
 From iris.proofmode Require Import tactics.
 From simuliris.simulation Require Import slsls lifting.
-From simuliris.simulang Require Import lang notation tactics class_instances
-  proofmode log_rel_structural wf.
+From simuliris.simulang Require Import lang notation tactics
+  proofmode log_rel_structural wf behavior.
 From simuliris.simulang.na_inv Require Export inv.
 From simuliris.simulang.na_inv Require Import readonly_refl adequacy.
 From iris.prelude Require Import options.
