theories/simulang/simple_inv/examples/reorder_malloc.v
@@ -1,6 +1,6 @@
 From iris.proofmode Require Import tactics.
 From simuliris.simulation Require Import slsls lifting.
-From simuliris.simulang Require Import lang notation tactics class_instances.
+From simuliris.simulang Require Import lang notation proofmode behavior.
 From simuliris.simulang.simple_inv Require Import inv adequacy.
 From iris.prelude Require Import options.
 
